txn-data-consistency/Tapir_Falsification.thy
@@ -6,20 +6,6 @@ begin
 
 subsection \<open>Lemmas and Invariants\<close>
 
-lemma ext_map_neqE:
-  "\<lbrakk>(\<lambda>k. map (\<lambda>t. P k t) (l k)) \<noteq> (\<lambda>k. map (\<lambda>t. Q k t) (l k)); \<exists>k t. P k t \<noteq> Q k t \<Longrightarrow> thesis\<rbrakk> \<Longrightarrow> thesis"
-proof -
-  assume a1: "(\<lambda>k. map (P k) (l k)) \<noteq> (\<lambda>k. map (Q k) (l k))"
-  assume a2: "\<exists>k t. P k t \<noteq> Q k t \<Longrightarrow> thesis"
-  obtain aa :: 'a where
-    "map (P aa) (l aa) \<noteq> map (Q aa) (l aa)"
-    using a1 by metis
-  then show ?thesis
-    using a2 by metis
-qed
-
-
-
 
 subsection \<open>Refinement Attempt\<close>
 
@@ -36,7 +22,7 @@ next
   then have (*I: "invariants_list gs" and *) reach_s': "reach tapir gs'" by auto
   with p show "ET_SER.ET_ES: sim gs\<midarrow>med a\<rightarrow> sim gs'"
   proof (induction a)
-    case (Cl_Commit cl sn u'' F ts  r_map w_map)
+    case (Cl_Commit cl sn u'' F ts r_map w_map)
     show ?case 
     proof -
       { 
@@ -71,7 +57,7 @@ next
           show \<open>fp_property F (kvs_of_s gs) u''\<close>
           proof -
             have a: "\<And>k v. F k R = Some v \<Longrightarrow>
-              \<exists>t. svr_state (svrs gs k) (get_wtxn gs cl) = occ_s (Some (v, t)) (F k W)"
+              \<exists>t. svr_state (svrs gs k) (get_wtxn gs cl) = prepared ts (Some (v, t)) (F k W)"
               using cmt
               apply (auto simp add: cl_commit_def)
               by (smt UnI1 UnI2 eq_fst_iff map_option_eq_Some option.distinct(1))
@@ -102,49 +88,45 @@ next
         by (simp only: ET_SER.trans_ET_ES_eq tapir_trans s_trans.simps sim_def med.simps)
     qed
   next
-    case (Cl_Prep x1 x2 x3 x4)
+    case (Cl_Issue x1 x2 x3)
     then show ?case
-      apply (auto simp add: sim_def tapir_trans_defs)
-      by (rule ext, auto simp add: sim_defs split: svr_state.split)+
+      apply (auto simp add: sim_defs tapir_trans_defs)
+      by (rule ext, auto simp add: sim_defs split: svr_state.split option.split)
   next
     case (Cl_Read_Resp x1 x2 x3 x4)
     then show ?case
+      apply (auto simp add: sim_defs tapir_trans_defs)
+      by (rule ext, auto simp add: sim_defs split: svr_state.split option.split)
+  next
+    case (Cl_Prep x1 x2 x3 x4)
+    then show ?case
       apply (auto simp add: sim_def tapir_trans_defs)
-      by (rule ext, auto simp add: sim_defs split: svr_state.split)+
+      by (rule ext, auto simp add: sim_defs split: svr_state.split option.split)
   next
     case (Cl_Abort x)
     then show ?case
       apply (auto simp add: sim_def tapir_trans_defs)
-      by (rule ext, auto simp add: sim_defs split: svr_state.split)+
+      by (rule ext, auto simp add: sim_defs split: svr_state.split option.split)+
   next
     case (Cl_ReadyC x1 x2)
     then show ?case
-      apply (auto simp add: sim_defs tapir_trans_defs)
-      apply (rule ext, auto simp add: sim_defs split: svr_state.split) sorry
+      apply (auto simp add: sim_def tapir_trans_defs)
+      apply (rule ext, auto simp add: sim_defs split: svr_state.split option.split) sorry
   next
     case (Cl_ReadyA x1 x2)
     then show ?case
       apply (auto simp add: sim_def tapir_trans_defs)
-      by (rule ext, auto simp add: sim_defs split: svr_state.split)+
+      by (rule ext, auto simp add: sim_defs split: svr_state.split option.split)
   next
-    case (Prep x1 x2 x3 x4)
+    case (Read_Resp x1 x2 x3)
     then show ?case
       apply (auto simp add: sim_defs tapir_trans_defs)
-      subgoal apply (elim ext_map_neqE, auto)
-        (*apply (auto simp add: sim_defs split: svr_state.split_asm option.split_asm)
-        apply (smt (verit) fun_upd_other fun_upd_same svr_conf.select_convs(1) svr_conf.surjective
-            svr_conf.update_convs(1) svr_state.distinct(13) svr_state.distinct(3))
-        apply (smt (verit) fun_upd_other fun_upd_same svr_conf.select_convs(1) svr_conf.surjective
-            svr_conf.update_convs(1) svr_state.distinct(17) svr_state.distinct(7))*) sorry
-      sorry
+      apply (rule ext, auto split: svr_state.split) sorry
   next
-    case (OCCCheck x1 x2 x3 x4 x5 x6)
+    case (Prep x1 x2 x3 x4 x5)
     then show ?case sorry
   next
-    case (CommitR x1 x2 x3 x4)
-    then show ?case sorry
-  next
-    case (CommitW x1 x2 x3 x4)
+    case (Commit x1 x2 x3 x4 x5)
     then show ?case sorry
   next
     case (Abort x1 x2)
